activity rules for dynamic auctions

isabelle/Auction/Sandbox/Trust.thy
@@ -18,7 +18,8 @@ Predicate
 (* "~~/src/HOL/Library/Code_Binary_Nat" *)
 "~~/src/HOL/Library/Code_Numeral"
 "~~/src/HOL/Library/Code_Char"
-
+"~~/src/HOL/UNITY/ListOrder"
+"~~/src/HOL/Library/Formal_Power_Series"
 begin
 
 abbreviation "currentBidder l == (size l - (2::nat)) mod (l!0)" (* the first bidder has label 0 *)
@@ -122,12 +123,99 @@ def main(args: Array[String]) {
 It can't probably get thinner than this.
 My ambition would be to handle everything besides input/output from inside Isabelle, including
 conversion from strings (as from input) to numbers and viceversa (for output); 
-this is definitely possible, but how realistic giving our schedule?
+this is definitely possible, but how realistic given our schedule?
 We could momentarily choose to directly use Scala integers as input/output, 
 which is less robust/flexible/elegant but simpler.
 *)
 
 export_code fst snd evaluateMe in Scala module_name a file "/dev/shm/a.scala"
-term liveliness
+
+find_consts "real set => real"
+term listrel
+value "maxpositions [1::nat,3, 2,3]"
+
+abbreviation "sublistAccordingTo list boolList == sublist list (set (filterpositions2 (%x. x=True) boolList))"
+value "sublistAccordingTo [1,2,3::int] [True,False,True]"
+
+fun valid where "valid step [] = []" |
+"valid step (x#xs) = (
+(card((set (maxpositions (sublistAccordingTo xs (valid step xs))))) \<ge> 2 & (x=Max (set 
+(sublistAccordingTo xs (valid step xs))
+))) 
+\<or>
+(card((set (maxpositions (sublistAccordingTo xs (valid step xs))))) = 1 & (x\<ge>Max (set 
+(sublistAccordingTo xs (valid step xs))
+) + step))
+\<or>
+(xs = [] & (x \<ge> 0))
+
+)#(valid step xs)"
+value "card((set (maxpositions [1::int,2,3,2,3]))) \<ge> 1"
+value "valid (-1::int) [1, 2, 3, 4]"
+
+abbreviation "isGrowing step l == (\<forall>n\<in>{0..<size l}. l!(Suc n) - (l!n)\<ge>step)"
+
+abbreviation "pairWise Op l m == [Op (l!i) (m!i). i <- [0..<min (size l) (size m)]]"
+lemma lm01: assumes "n\<in>{0..<min (size l) (size m)}" shows "(pairWise Op l m)!n = Op (l!n) (m!n)"
+using assms by auto
+abbreviation "deltaBids (*step*) l == (* step # *) (pairWise (op -) (tl l) l)"
+value "filterpositions2 (%x. x>3) [1::nat,2]"
+lemma lm02: "min (size (tl l)) (size l)=size l - (1::nat)" by simp
+lemma lm03: assumes "n\<in>{0..<size (l::int list)-(1::nat)}" shows "(deltaBids l)!n=(l!(Suc n)) - ((l!n)::int)" using 
+assms lm02 length_tl nth_tl atLeastLessThan_iff diff_zero monoid_add_class.add.left_neutral 
+nth_map_upt by (metis (erased, lifting))
+abbreviation "firstInvalidBidIndex step l == 
+1 + hd (filterpositions2 (%x. x<step) (deltaBids (*step*) l)@[size l])"
+
+lemma fixes f::"nat => real" shows "setsum (%x. f (x+1) - f x) {0..<Suc n}=f (Suc n) - f 0"
+using assms setsum_natinterval_difff setsum_Suc_diff sorry
+
+
+lemma assumes "size (l::int list)\<ge>2" shows "listsum [l!(n+1)-(l!n). n<-[0..<size l - (1::nat)]]=l!(size l - (1::nat))-(l!0)"
+using assms setsum_natinterval_difff setsum_Suc_diff sorry
+
+lemma assumes "size l\<ge>2" shows "l!(size l-(1::nat))=listsum (deltaBids l) + ((l!0)::int)"
+using assms lm03 sorry
+
+abbreviation "amendedbidlist3 step l == update2 l {firstInvalidBidIndex step l..<size l} (%x. 
+l!(firstInvalidBidIndex step l - 1))"
+
+lemma assumes "step \<ge>(1::nat)" "firstInvalidBidIndex step (l::nat list)=Suc 0" shows 
+"l!0 \<ge> 0*step" using assms by presburger
+
+lemma assumes "step \<ge>(1::nat)" "firstInvalidBidIndex step (l::nat list)=Suc (Suc n)"
+"\<forall>m\<le>n. firstInvalidBidIndex step (l::nat list)=Suc m \<longrightarrow> l!m\<ge>m*step" shows
+"l!(Suc n)\<ge>(Suc n)*step" using assms filterpositions2_def sorry
+
+lemma assumes "l\<noteq>[]" "step \<ge>(1::nat)" "firstInvalidBidIndex step (l::nat list)=Suc n" shows 
+"!m<n. (deltaBids l)!m \<ge> step " using assms nth_def using filterpositions2_def sorry
+
+lemma assumes "step \<ge>(1::nat)" "firstInvalidBidIndex step (l::nat list)=Suc n" shows 
+"l!n \<ge> n*step + (l!0)" using assms filterpositions2_def lm01 lm02 lm03 
+setsum_natinterval_difff setsum_Suc_diff sorry
+
+
+abbreviation "EX02 == [0::nat, 2, 4, 6, 8, 11, 12, 11]"
+value "firstInvalidBidIndex 2 EX02"
+value "amendedbidlist3 2 EX02"
+
+abbreviation "setOfAllowedBids step l == {x. x=Max (set l) \<or> (isGrowing step l \<and> x \<ge> step+Max (set l))}"
+value "Example02"
+value "amendedbidlist (Example02,,20)"
+
+lemma assumes "(step::nat) \<ge> 1" "\<forall>l\<in>(X::nat list set). set l \<subseteq> {0..0}" shows "EX n. \<forall>l. l \<in> X \<longrightarrow> firstInvalidBidIndex step l < n" 
+using assms 
+using filterpositions2_def sorry
+
+lemma assumes "(step::nat) \<ge> 1" "\<forall>l\<in>(X::nat list set). set l \<subseteq> {0..N}" shows "EX n. \<forall>l. l \<in> X \<longrightarrow> firstInvalidBidIndex step l < n"
+using assms 
+unfolding filterpositions2_def
+
+lemma assumes "\<forall>l\<in>X. set l \<subseteq> {0..N}" 
+shows "EX M n. \<forall> l\<in> X. (\<forall>m. (m > n & m < size l) \<longrightarrow> ((amendedbidlist3 step l)!m = M))"
+using assms sorry
+
+(* abbreviation "allowedBids bidSet bid == " activity rule*)
+
 end
 
